

Least Square fit for a straight line

Compiled and Designed by Sai Satyapriya

$$E = \sum_{i=1}^n [y_i - f(x_i)]^2$$

Here,

$$f(x_i) = mx_i + c$$

$$E = \sum_{i=1}^n [y_i - (mx_i + c)]^2$$

or

$$E = \sum_{i=1}^n [y_i - mx_i - c]^2$$

$$\frac{\partial E}{\partial m} = 2 \sum_{i=1}^n [y_i - mx_i - c] (-x_i) = 0$$

$$\Rightarrow \sum y_i x_i - m \sum x_i^2 - c \sum x_i = 0$$

$$\boxed{m \sum x_i^2 + c \sum x_i = \sum y_i x_i}$$

—

$$\frac{\partial E}{\partial c} = 2 \sum_{i=1}^n [y_i - mx_i - c] (-1) = 0$$

$$\Rightarrow \sum y_i - m \sum x_i - c \sum 1 = 0$$

$$\boxed{m \sum x_i + cN = \sum y_i}$$

—

Matrix form

$$\begin{bmatrix} \sum x_i^2 & \sum x_i \\ \sum x_i & N \end{bmatrix} \begin{bmatrix} m \\ c \end{bmatrix} = \begin{bmatrix} \sum y_i x_i \\ \sum y_i \end{bmatrix}$$

—

Solution

$$\begin{bmatrix} m \\ c \end{bmatrix} = \begin{bmatrix} \sum x_i^2 & \sum x_i \\ \sum x_i & N \end{bmatrix}^{-1} \begin{bmatrix} \sum y_i x_i \\ \sum y_i \end{bmatrix}$$

—